\documentclass{scrartcl}
\usepackage{mathtools}

\begin{document}
    For \(y = Ax\), prove that
    \begin{itemize}
        \item \(E[y] = AE[x]\)
        \item \(A cov(x) A^{T}\)
    \end{itemize}

    \begin{align*}
        \textnormal{cov}[y] &= E[(y - E(y))(y - E(y))^\textnormal{T}]\\
        &= E[(Ax-AE[x])(Ax-AE(x))^\textnormal{T}]\\
        &= E[A(x-E[x])(x-E[x])^\textnormal{T}A^\textnormal{T}]\\
        &= AE[(x-E[x])(x-E[x])^\textnormal{T}]A^\textnormal{T}\\
        &= A\textnormal{cov}[x]A^\textnormal{T}
    \end{align*}
\end{document}
